---
title: "Documento Completo"
topic: "General"
number: "1"
originalUrl: "exports/downloads/Todos los ramos/I3 2022-2_3lP5bwZ4F95Pc7Gps7rR.pdf"
sourceFile: "I3 2022-2_3lP5bwZ4F95Pc7Gps7rR.pdf"
---

--- Page 1 ---
★  𝑓 ( 𝑥 ,   𝑦 ,   𝑧 )   =   𝑦𝑧  𝑥  𝑓 ( 𝑥 ,   𝑦 ,   𝑧 )   =   6  𝑃 ( 1 , 2 , 3 )  ∇ 𝑓 ( 𝑥 ,   𝑦 ,   𝑧 )   =   −   𝑦𝑧  𝑥 2   𝑖 ⃗   +   𝑧  𝑥   𝑗 ⃗   +   𝑦  𝑧   𝑘 ⃗ ⃗  𝑃 ( 1 , 2 , 3 )  𝑛 ⃗ ⃗   =   ∇ 𝑓 ( 1 , 2 , 3 )   =   − 6 𝑖 ⃗   +   3 𝑗 ⃗   +   2 𝑘 ⃗ ⃗  − 6 ( 𝑥   −   1 )   +   3 ( 𝑦   −   2 )   +   2 ( 𝑧   −   3 )   =   0  𝑢 ⃗ ⃗   =   𝑖 ⃗   +   𝑐 𝑗 ⃗   −   𝑐 𝑘 ⃗ ⃗   𝑐   𝑐  𝐷𝑓 𝑢 ⃗ ⃗ ⃗   ( 𝑃 )   =   0  ( 𝐷 𝑢 ⃗ ⃗ ⃗   𝑓 ) ( 𝑃 )   =   ∇ 𝑓 ( 1 , 2 , 3 )   ⋅   𝑢 ⃗ ⃗  =   ( − 6 𝑖 ⃗   +   3 𝑗 ⃗   +   2 𝑘 ⃗ ⃗   )   ⋅   ( 𝑖 ⃗   +   𝑐 𝑗 ⃗   −   𝑐 𝑘 ⃗ ⃗   )  =   − 6   +   𝑐  𝑐   =   6

--- Page 2 ---
𝑓 ( 𝑥 ,   𝑦 )   =   𝑥 2 𝑦   +   𝑥 𝑦 2  𝑔 ( 𝑠 ,   𝑡 )   =   ( 𝑥 ( 𝑠 ,   𝑡 ) ,   𝑦 ( 𝑠 ,   𝑡 ) )   =   ( 𝑡   −   2 ,   𝑠𝑡 )  ∂ ℎ  ∂ 𝑠   ( 1 , 2 )  ℎ ( 𝑠 ,   𝑡 )   =   𝑓 ( 𝑥 ( 𝑠 ,   𝑡 ) ,   𝑦 ( 𝑠 ,   𝑡 ) )  ∂ ℎ  ∂ 𝑠   ( 𝑠 ,   𝑡 )   =   ∂ 𝑓  ∂ 𝑥   ( 𝑥 ,   𝑦 )   ∂ 𝑥  ∂ 𝑠   ( 𝑠 ,   𝑡 )   +   ∂ 𝑓  ∂ 𝑦   ( 𝑥 ,   𝑦 )   ∂ 𝑦  ∂ 𝑠   ( 𝑠 ,   𝑡 )  ( 𝑠 ,   𝑡 )   =   ( 1 , 2 ) ,   ( 𝑥 ,   𝑦 )   =   ( 2   −   2 , 1   ⋅   2 )   =   ( 0 , 2 )  ∂ 𝑓  ∂ 𝑥   =   2 𝑥𝑦   +   𝑦 2 ;   ∂ 𝑓  ∂ 𝑥   ( 0 , 2 )   =   4  ∂ 𝑓  ∂ 𝑥   =   𝑥 2   +   2 𝑥𝑦 ;   ∂ 𝑓  ∂ 𝑦   ( 0 , 2 )   =   0  𝜕𝑥  𝜕𝑠   =   0 ;   𝜕𝑥  𝜕𝑠   ( 1 , 2 )   =   0  𝜕𝑦  𝜕𝑠   =   𝑡 ;   𝜕𝑦  𝜕𝑠   ( 1 , 2 )   =   2  ∂ ℎ  ∂ 𝑠   ( 1 , 2 )   =   ∂ 𝑓  ∂ 𝑥   ( 0 , 2 )   ∂ 𝑥  ∂ 𝑠   ( 1 , 2 )   +   ∂ 𝑓  ∂ 𝑦   ( 0 , 2 )   ∂ 𝑦  ∂ 𝑠   ( 1 , 2 )  =   4   ⋅   0   +   0   ⋅   2  =   0

--- Page 3 ---
( 𝑥 ,   𝑦 )  𝑇 ( 𝑥 ,   𝑦 )   =   30 𝑒 − ( 𝑥 2 + 4 𝑦 2 )  𝑇  30 𝑒 − ( 𝑥 2 + 4 𝑦 2 )   𝑥 2   +   4 𝑦 2  𝑥 2   +   4 𝑦 2   =   𝑐  𝑥 2  √ 𝑐 2   +   𝑦 2  ( √ 𝑐  2   )  2   =   1  ( 0 , 0 )   𝑥  𝑦  ∇ 𝑇 ( 𝑥 ,   𝑦 )  ∇ 𝑇 ( 𝑥 ,   𝑦 )   =   ⟨ 𝑇 𝑥 ,   𝑇 𝑦 ⟩   =   ⟨ − 60 𝑥 𝑒 − ( 𝑥 2 + 4 𝑦 2 ) ,   − 240 𝑦 𝑒 − ( 𝑥 2 + 4 𝑦 2 ) ⟩  ( 1 , 1 )  ∇ 𝑇 ( 1 , 1 )   =   ⟨ − 60 𝑒 − 5 ,   − 240 𝑒 − 5 ⟩  ⟨ − 1 ,   − 4 ⟩

--- Page 4 ---
𝑓 ( 𝑥 ,   𝑦 )   =   𝑥 2 𝑦   −   𝑥 2   −   2 𝑦 2  𝑓 𝑥   =   2 𝑥𝑦   −   2 𝑥   𝑓 𝑦   =   𝑥 2   −   4 𝑦  { 2 𝑥𝑦   −   2 𝑥   =   0  𝑥 2   −   4 𝑦   =   0  𝑥   =   0   𝑦   =   1   𝑦   =   0   𝑥   =   ± 2  ( 0 , 0 ) ,   ( − 2 , 1 ) ,   ( 2 , 1 )  𝑓 𝑥𝑥   =   2 𝑦   −   2 ,   𝑓 𝑥𝑦   =   2 𝑥 ,   𝑓 𝑦𝑦   =   − 4  𝐷   =   − 8 𝑦   +   8   −   4 𝑥 2  •   ( 0 , 0 )   𝑓 𝑥𝑥   =   − 2   <   0   𝐷   =   8   𝑓  •   ( ± 2 , 1 )   𝐷   =   − 16   𝑓

--- Page 5 ---
𝑧   =   8 𝑥   −   𝑦   𝑃 ( 9 , 4 , 2 )  𝑓 ( 𝑥 ,   𝑦 ,   𝑧 )   =   distancia ( ( 𝑥 ,   𝑦 ,   𝑧 ) ,   ( 9 , 4 , 2 ) ) 2   =   ( 𝑥   −   9 ) 2   +   ( 𝑦   −   4 ) 2   +   ( 𝑧   −   2 ) 2  𝑔 ( 𝑥 ,   𝑦 ,   𝑧 )   =   8 𝑥   −   𝑦   −   𝑧  ∇ 𝑓   =   λ ∇ 𝑔   8 𝑥   −   𝑦   =   𝑧  {  2 ( 𝑥   −   9 )   =   8 𝜆  2 ( 𝑦   −   4 )   =   − 𝜆  2 ( 𝑧   −   2 )   =   − 𝜆  8 𝑥   −   𝑦   =   𝑧  𝜆  {  2 ( 𝑥   −   9 )   =   8 𝜆   →   𝜆   =   1  4   ( 𝑥   −   9 )  2 ( 𝑦   −   4 )   =   − 𝜆   →   𝜆   =   − 2 ( 𝑦   −   4 )  2 ( 𝑧   −   2 )   =   − 𝜆   →   𝜆   =   − 2 ( 𝑧   −   2 )  8 𝑥   −   𝑦   =   𝑧  1  4   ( 𝑥   −   9 )   =   − 2 ( 𝑦   −   4 )   =   − 2 ( 𝑧   −   2 )  𝑦   =   𝑧   +   2 ,   𝑥   =   − 8 𝑧   +   25  8 𝑥   −   𝑦   =   𝑧  {  𝑧   =   8 ( − 8 𝑧   +   25 )   −   𝑧   −   2   →   𝑧   =   3  𝑦   =   3   +   2   =   5  𝑥   =   − 8   ∙   3   +   25   =   1  ( 1 , 5 , 3 )

--- Page 6 ---
𝑓 ( 𝑥 ,   𝑦 )   =   3   +   𝑥𝑦   −   𝑥   −   𝑦  𝐷  𝐴 ( 0 , 0 )   𝐵 ( 1 , 0 )   𝐶 ( 0 , 1 )  𝐷  ∇ 𝑓   =   ⟨ 𝑦   −   1 ,   𝑥   −   1 ⟩   =   0   →   𝑦   =   1 ,   𝑥   =   1  ( 1 , 1 )  •   𝑥   =   0   0   ≤   𝑦   ≤   1   𝐴𝐶 ̅ ̅ ̅ ̅  𝑓 ( 0 ,   𝑦 )   =   𝑓 1 ( 𝑦 )   =   3   −   𝑦  𝑓 1  ′ ( 𝑦 )   =   − 1   ≠   0  𝑓 ( 0 , 0 )   =   𝑓 1 ( 0 )   =   3 ,   𝑓 ( 0 , 1 )   =   𝑓 1 ( 1 )   =   2  •   𝑦   =   0   0   ≤   𝑥   ≤   1   𝐴𝐵 ̅ ̅ ̅ ̅  𝑓 ( 𝑥 ,   0 )   =   𝑓 2 ( 𝑥 )   =   3   −   𝑥  𝑓 2  ′ ( 𝑥 )   =   − 1   ≠   0  𝑓 ( 0 , 0 )   =   𝑓 2 ( 0 )   =   3 ,   𝑓 ( 1 , 0 )   =   𝑓 2 ( 1 )   =   2

--- Page 7 ---
•   𝑦   =   1   −   𝑥   0   ≤   𝑥   ≤   1   𝐶𝐵 ̅ ̅ ̅ ̅  f ( 𝑥 ,   1   −   𝑥 )   =   𝑓 3 ( 𝑥 )   =   3   +   𝑥 ( 1   −   𝑥 )   −   𝑥   −   ( 1   −   𝑥 )   =   2   +   𝑥   −   𝑥 2  𝑓 3  ′ ( 𝑥 )   =   1   −   2 𝑥   𝑥   =   1  2  ( 1  2   ,   1  2 )  𝑓   ( 1  2   ,   1  2 )   =   𝑓 3   ( 1  2   ,   1  2 )   =   2   +   1  4  𝑓 ( 0 , 1 )   =   𝑓 3 ( 0 )   =   3 ,   𝑓 ( 1 , 0 )   =   𝑓 3 ( 1 )   =   2  𝑓  ( 0 , 0 )   3   ( 1 , 0 )  ( 0 , 1 )   2

