---
title: "Ejercicio 2"
topic: "General"
number: "2"
originalUrl: "exports/downloads/Todos los ramos/Ayudantia6_Solucionario_26ztlX7IBvC9aU5h8dis.pdf"
sourceFile: "Ayudantia6_Solucionario_26ztlX7IBvC9aU5h8dis.pdf"
---

Para cada una de las siguientes funciones, determine   y ′ , usando la derivaci´ on logar´ ıtmica. (a)   y   = (tan( x ))   1  x  (b)   y   =   e x 2 − x   cos 2 ( x )  3  √ ( x   + 1) 2  Soluci´ on:  (a)  y   = (tan( x ))   1  x   ⇒   ln ( y ) = ln  (  (tan( x ))   1  x  )  ⇒   ln ( y ) =  1  x   ln (tan( x ))  ⇒   d dx   ln ( y ) =   d dx  (   1  x   ln (tan( x ))  )  ⇒   y ′  y   =   −   1  x 2   ln (tan( x )) +  1  x  sec 2 ( x ) tan( x )  ⇒   y ′   =   y  (  −   1  x 2   ln (tan( x )) +  sec 2 ( x )  x   tan( x )  )  ⇒   y ′   = (tan( x ))   1  x  (  −   1  x 2   ln (tan( x )) +  sec 2 ( x )  x   tan( x )  )  (b)  y   =   e x 2 − x   cos 2 ( x )  3  √ ( x   + 1) 2   ⇒   ln ( y ) = ln  (  e x 2 − x   cos 2 ( x )  3  √ ( x   + 1) 2  )  ⇒   ln ( y ) = ln  (  e x 2 − x   cos 2 ( x )  )  −   ln  (   3  √ ( x   + 1) 2  )  ⇒   ln ( y ) = ln  (  e x 2 − x  )  + ln   ( cos 2 ( x ) )   −   2 3  ln (( x   + 1))  ⇒   ln ( y ) = ln  (  e x 2 − x  )  + 2 ln (cos( x ))   −   2 3  ln (( x   + 1))  ⇒   ln ( y ) =   x 2   −   x   + 2 ln (cos( x ))   −   2 3  ln ( x   + 1)  ⇒   y ′  y   = 2 x   −   1   −   2 sen( x ) cos( x )   −   2 3( x   + 1)  ⇒   y ′   =   y  (  2 x   −   1   −   2 tan( x )   −   2 3( x   + 1)  )  ⇒   y ′   =  (  e x 2 − x   cos 2 ( x )  3  √ ( x   + 1) 2  )  (  2 x   −   1   −   2 tan( x )   −   2 3( x   + 1)  )

--- Page 3 ---