Utilice la derivaci´ on impl´ ıcita para calcular la derivada indicada. (a)   dy dx   si arctan ( x 2 y ) =   x   +   xy 2  (b)   dx dy   si   y   sec( x ) =   x   tan( y )  Soluci´ on:  (a) arctan   ( x 2 y )   =   x   +   xy 2   ⇒   d dx   arctan   ( x 2 y )   =   d dx  ( x   +   xy 2 )  ⇒   2 xy   +   x 2   dy dx  1 +   x 4 y 2   = 1 +   y 2   + 2 xy  dy dx  ⇒   dy dx  (   x 2  1 +   x 4 y 2   −   2 xy  )  = 1 +   y 2   −   2 xy  1 +   x 4 y 2  ⇒   dy dx   =  (1 +   y 2 ) (1 +   x 4 y 2 )   −   2 xy x 2   −   2 xy   (1 +   x 4 y 2 ) (b)  y   sec( x ) =   x   tan( y )   ⇒   d dy   ( y   sec( x )) =   d dy   ( x   tan( y ))  ⇒   sec( x ) +   y   sec( x ) tan( x ) dx dy   =   dx dy   tan( y ) +   x   sec 2 ( y )  ⇒   dx dy   ( y   sec( x ) tan( x )   −   tan( y )) =   x   sec 2 ( y )   −   sec( x )  ⇒   dx dy   =   x   sec 2 ( y )   −   sec( x )  y   sec( x ) tan( x )   −   tan( y )

--- Page 4 ---