---
title: "Ejercicio 5"
topic: "General"
number: "5"
originalUrl: "exports/downloads/Todos los ramos/I2 2016-2_0KETG37itRHP5Xpzvjgt.pdf"
sourceFile: "I2 2016-2_0KETG37itRHP5Xpzvjgt.pdf"
---

Si   z   =   f   ( x, y ), donde   x   =   r 2   +   s 2 ,   y   = 2 rs , determine   ∂ 2 z  ∂r∂s   .  Soluci´ on. Usando la regla de la cadena se tiene  ∂z  ∂s   =   ∂z  ∂x ∂x  ∂s   +   ∂z  ∂y ∂y  ∂s   =   ∂z  ∂x   2 s   +   ∂z  ∂y   2 r .  Entonces, aplicando la regla del producto y la regla de la cadena se obtiene  ∂ 2 z  ∂r∂s   =   ∂  ∂r  (   ∂z  ∂x   2 s  )  +   ∂  ∂r  (   ∂z  ∂y   2 r  )  =   ∂ 2 z  ∂x 2  ∂x  ∂r   2 s   +   ∂  ∂y  (   ∂z  ∂x  )   ∂y  ∂r   2 s   +   ∂z  ∂x ∂  ∂r   (2 s ) +   ∂ 2 z  ∂y 2  ∂y  ∂r   2 r   +   ∂  ∂x  (   ∂z  ∂y  )   ∂x  ∂r   2 r   +   ∂z  ∂y   2 =   4 rs  ∂ 2 z  ∂x 2   +   ∂ 2 z  ∂y∂x   4 s 2   + 4 rs  ∂ 2 z  ∂y 2   +   ∂ 2 z  ∂x∂y   4 r 2   + 2   ∂z  ∂y  =   4 rs  ∂ 2 z  ∂x 2   + 4 rs  ∂ 2 z  ∂y 2   + (4 r 2   + 4 s 2 )   ∂ 2 z  ∂x∂y   + 2   ∂z  ∂y  .

--- Page 6 ---